Scratch2.thy
@@ -2,92 +2,29 @@ theory Scratch2
 imports RHL_Typed Hoare_Tactics Procs_Typed Tactic_Inline 
 begin
 
-definition "HIDDEN_EQ = op="
-lemma HIDDEN_EQ_refl: "HIDDEN_EQ x x" unfolding HIDDEN_EQ_def ..
-lemma HIDDEN_EQ_procargs:
-  shows "HIDDEN_EQ procargvars_empty procargvars_empty"
-    and "HIDDEN_EQ a b \<Longrightarrow> HIDDEN_EQ (procargvars_add (LVariable x) a) (procargvars_add (LVariable x) b)"
-unfolding HIDDEN_EQ_def by auto
-lemma HIDDEN_EQ_varset:
-  fixes x x' y y'
-  defines "x == mk_variable_untyped (LVariable x')"
-  defines "y == mk_variable_untyped (Variable y')"
-  shows "HIDDEN_EQ {} {}"
-    and "HIDDEN_EQ a b \<Longrightarrow> HIDDEN_EQ (Set.insert x a) (Set.insert x b)"
-    and "HIDDEN_EQ a b \<Longrightarrow> HIDDEN_EQ (Set.insert y a) (Set.insert y b)"
-    and "HIDDEN_EQ a b \<Longrightarrow> HIDDEN_EQ a' b' \<Longrightarrow> HIDDEN_EQ (a \<union> a') (b \<union> b')"
-unfolding HIDDEN_EQ_def by auto
-lemma HIDDEN_EQ_I': "HIDDEN_EQ a b \<Longrightarrow> a==b" by (simp add: HIDDEN_EQ_def)
-lemma HIDDEN_EQ_D': "a==b \<Longrightarrow> HIDDEN_EQ a b" by (simp add: HIDDEN_EQ_def)
-
-lemma vars_proc_global_inter_vu_global: 
-  "set (vars_proc_global f) \<inter> Collect vu_global = set (vars_proc_global f)"
-unfolding vars_proc_global_def by auto
-
-abbreviation "globVar == Variable ''globVar''"
+ML {* @{term "1==1"} *}
 
 
-lemma filter_locals1: "Set.filter (\<lambda>x. \<not> vu_global x) (insert (mk_variable_untyped (LVariable x :: 'a::prog_type variable)) V)
-  = insert (mk_variable_untyped (LVariable x :: 'a variable)) (Set.filter (\<lambda>x. \<not> vu_global x) V)"
-  by auto
-lemma filter_locals2: "Set.filter (\<lambda>x. \<not> vu_global x) (insert (mk_variable_untyped (Variable x :: 'a::prog_type variable)) V)
-  = Set.filter (\<lambda>x. \<not> vu_global x) V"
-  by auto
-lemma filter_locals3: "Set.filter (\<lambda>x. \<not> vu_global x) (set (vars_proc_global f)) = {}"
-  using vars_proc_global_inter_vu_global by fastforce 
+ML "Binding.empty"
 
-procedure testproc :: "(unit,unit) procedure \<Rightarrow> (int*unit,int)procedure" where
-  "testproc f = LOCAL x y a z. proc(a) {x:=a; z:=call f(); y:=(1::int); globVar:=x; return x+y;}"
-schematic_lemma testproc_body [procedure_info]: "p_body (testproc f) == ?b" unfolding testproc_def by simp
-schematic_lemma testproc_return [procedure_info]: "p_return (testproc f) == ?b" unfolding testproc_def by simp
-schematic_lemma testproc_args [procedure_info]: "p_arg (testproc f) == ?b" unfolding testproc_def by simp
-schematic_lemma testproc_body_vars [procedure_info]: "set (vars_proc_global f) == fv \<Longrightarrow> set (vars (p_body (testproc f))) == ?b" unfolding testproc_body by simp
-schematic_lemma testproc_body_local_vars [procedure_info]: "set (local_vars (p_body (testproc f))) == ?b" 
- apply (rule HIDDEN_EQ_I')
- unfolding local_vars_def filter_set[symmetric] apply (subst testproc_body_vars) apply simp_all
- unfolding filter_locals1 filter_locals2 filter_locals3
- by (rule HIDDEN_EQ_varset)+
-schematic_lemma testproc_body_vars': "set (vars (p_body (testproc f))) == ?b" by (subst testproc_body_vars, simp, simp)
-schematic_lemma testproc_global_vars [procedure_info]: assumes "set (vars_proc_global f) == fv" shows "set (vars_proc_global (testproc f)) == ?b" 
- apply (rule HIDDEN_EQ_I')
- unfolding vars_proc_global_def testproc_body testproc_return 
- apply (simp add: vars_proc_global_inter_vu_global)
- unfolding assms
- by (rule HIDDEN_EQ_varset HIDDEN_EQ_refl[of fv])+
-schematic_lemma testproc_global_vars': "set (vars_proc_global (testproc f)) == ?b" by (subst testproc_global_vars, simp, simp)
-schematic_lemma testproc_return_vars [procedure_info]: "set (e_vars (p_return (testproc f))) == ?b" unfolding testproc_return by simp
-
-
-
-section "MODULE TYPE"
-
-type_synonym 'a testmodule_rep = "(('a*unit,unit)procedure * (unit,'a) procedure)"
-
-typedef 'a testmodule = "UNIV::'a testmodule_rep set" by auto
-
-instantiation testmodule :: (prog_type)procedure_functor begin
-definition "procedure_functor_type (_::'a testmodule itself) == procedure_functor_type (TYPE('a testmodule_rep))"
-definition "procedure_functor_mk_untyped x == procedure_functor_mk_untyped (Rep_testmodule x)"
-definition "procedure_functor_mk_typed' p == Abs_testmodule (procedure_functor_mk_typed' p)"
-instance 
-  apply intro_classes
-  close (unfold procedure_functor_mk_untyped_testmodule_def procedure_functor_type_testmodule_def, fact procedure_functor_welltyped)
-  close (unfold procedure_functor_mk_untyped_testmodule_def, fact procedure_functor_beta_reduced)
-  close (unfold procedure_functor_mk_untyped_testmodule_def procedure_functor_mk_typed'_testmodule_def procedure_functor_type_testmodule_def Abs_testmodule_inverse[OF Set.UNIV_I],
-         fact procedure_functor_mk_typed_inverse')
-  apply (unfold procedure_functor_mk_typed'_testmodule_def procedure_functor_mk_untyped_testmodule_def Rep_testmodule_inverse procedure_functor_mk_untyped_inverse')
-  by (fact refl)
+local_setup {*
+fn ctx => 
+let val tac = ALLGOALS (simp_tac ctx)
+    val method : Method.text = tac
+                 |> SIMPLE_METHOD |> K |> Method.Basic
+    fun eq_sch n t = Logic.mk_implies (Logic.mk_equals (Free(n,@{typ int}), Var((n,0),@{typ int})), t)
+    val st = Proof.theorem NONE (fn thms => fn ctx => (@{print} thms; ctx)) 
+      [[(eq_sch "X" @{prop "X==1+0+0::int"},[])],[(eq_sch "X" @{prop "X==1+0::int"},[])]] ctx
+    val st' = Proof.apply method st |> Seq.hd
+    val ctx = Proof.global_done_proof st'
+in
+ctx
 end
+*}
 
-term testmodule
-
-definition "proc1 module = (case module of (proc1_,proc2_) \<Rightarrow> proc1_)"
-definition "proc2 module = (case module of (proc1_,proc2_) \<Rightarrow> proc2_)"
-definition "testmodule x_proc1 x_proc2 == Abs_testmodule (x_proc1,x_proc2)"
-
-term "x::int testmodule == y::_::procedure_functor"
-
-
-
+schematic_lemma
+  assumes "X = ?X"
+  shows "X = 1"
+  and "X = 2"
 
 end
